aneris/examples/reliable_communication/lib/reliable_rpc/api_spec.v
@@ -13,10 +13,10 @@ Section Spec.
 	Context (srv_si : message → iProp Σ).
 	Notation srv_ip := (ip_of_address RPC_saddr).
 
-	Context (LockedChannel : val → socket_address → iProp Σ).
+	Context (Channel : val → socket_address → iProp Σ).
 
 	Definition implement_spec {RP : RPC_rpc_params} (IMP : RPC_implementation_params RP) : iProp Σ :=
-		{{{ ⌜In RP IP⌝ }}}
+		{{{ ⌜In RP IP.(RPC_inter)⌝ }}}
 			implement IMP.(RPC_val) IMP.(RPC_handler) @[srv_ip]
 		{{{ h, RET (#RP.(RPC_name), h)%V; ⌜is_impl_handler_of_rpc h RP⌝ }}}.
 
@@ -29,7 +29,7 @@ Section Spec.
 				free_ports (srv_ip) {[port_of_address RPC_saddr]} ∗
 				SrvInit }}}
 			init_server_stub #RPC_saddr II.(RPC_inter_val) @[srv_ip]
-		{{{ RET #(); ⌜True⌝ }}}.
+		{{{ RET #(); ⌜False⌝ }}}.
 
 	Definition init_client_stub_spec : iProp Σ :=
 		∀ A clt_addr,
@@ -39,19 +39,30 @@ Section Spec.
 				clt_addr ⤳ (∅, ∅) ∗
 				free_ports (ip_of_address clt_addr) {[port_of_address clt_addr]} }}}
 			init_client_stub #clt_addr #RPC_saddr @[ip_of_address clt_addr]
-		{{{ chan, RET chan; LockedChannel chan clt_addr }}}.
+		{{{ chan, RET chan; Channel chan clt_addr }}}.
 
-	Definition rpc_spec {RP : RPC_rpc_params} (f : val) clt_addr : iProp Σ :=
+	Definition call_spec {RP : RPC_rpc_params} (IMP : RPC_implementation_params RP) : iProp Σ :=
+		∀ chan clt_addr argv argd,
+		{{{ ⌜In RP IP.(RPC_inter)⌝ ∗ 
+			Channel chan clt_addr ∗
+			⌜Serializable RP.(RPC_arg_ser) argv⌝ ∗ 
+			RP.(RPC_pre) argv argd }}}
+			call chan IMP.(RPC_val) argv @[ip_of_address clt_addr]
+		{{{ repv repd, RET repv; 
+			Channel chan clt_addr ∗
+			RP.(RPC_post) repv argd repd }}}.
+
+	(* Definition rpc_spec {RP : RPC_rpc_params} (f : val) clt_addr : iProp Σ :=
 		∀ argv argd,
-		{{{ RP.(RPC_pre) argv argd }}}
+		{{{ ⌜Serializable RP.(RPC_arg_ser) argv⌝ ∗ RP.(RPC_pre) argv argd }}}
 			f argv @[ip_of_address clt_addr]
 		{{{ repv repd, RET repv; RP.(RPC_post) repv argd repd }}}.
 
 	Definition call_spec {RP : RPC_rpc_params} (IMP : RPC_implementation_params RP) : iProp Σ :=
 		∀ chan clt_addr,
-		{{{ ⌜In RP IP⌝ ∗ LockedChannel chan clt_addr }}}
+		{{{ ⌜In RP IP.(RPC_inter)⌝ ∗ Channel chan clt_addr }}}
 			call chan IMP.(RPC_val) @[ip_of_address clt_addr]
-		{{{ f, RET f; @rpc_spec RP f clt_addr }}}.
+		{{{ f, RET f; @rpc_spec RP f clt_addr }}}. *)
 
 End Spec.
 
@@ -59,18 +70,18 @@ End Spec.
 Section RPC_Init.
 
 	Context `{ !anerisG Mdl Σ, !lockG Σ}.
-	Check call_spec.
+
 	Class RPC_init := {
 		RPC_init_setup E (UP : RPC_user_params) (IP : RPC_interface_params) :
 		↑RPC_mN ⊆ E →
     ⊢ |={E}=> ∃ (srv_si : message → iProp Σ) (SrvInit : iProp Σ)
-								(LockedChannel : val → socket_address → iProp Σ),
+								(Channel : val → socket_address → iProp Σ),
 			SrvInit ∗
 			(∀ (II : RPC_interface_implementation IP), 
 				init_server_stub_spec SrvInit srv_si II) ∗
-			(init_client_stub_spec srv_si LockedChannel) ∗
+			(init_client_stub_spec srv_si Channel) ∗
 			( ∀ (RP : RPC_rpc_params) (IMP : RPC_implementation_params RP),
-				@call_spec _ _ _ _ IP LockedChannel RP IMP)
+				@call_spec _ _ _ _ IP Channel RP IMP)
 	}.
 
-Section RPC_Init.
+End RPC_Init.
