aneris/examples/reliable_communication/lib/reliable_rpc/reliable_rpc_proof.v
@@ -1,7 +1,7 @@
 From iris.base_logic.lib Require Import invariants.
 From iris.proofmode Require Import coq_tactics reduction spec_patterns.
 From aneris.aneris_lang Require Import lang.
-From aneris.aneris_lang.lib Require Import lock_proof set_proof.
+From aneris.aneris_lang.lib Require Import lock_proof set_proof list_proof.
 From aneris.aneris_lang.lib.serialization Require Import serialization_proof.
 From aneris.aneris_lang Require Import tactics proofmode.
 From actris.channel Require Export proto.
@@ -14,22 +14,24 @@ From aneris.examples.reliable_communication.lib.reliable_rpc
 From aneris.examples.reliable_communication.prelude Require Import ser_inj.
 
 Import reliable_rpc_code.
-Import monitor_proof.
 Import lock_proof.
 Import client_server_code.
 
 Section RPC_proof_of_code.
 	Context `{ !anerisG Mdl Σ, !lockG Σ}.
 	Context `{ !RPC_user_params }.
-	Context (SrvInit : iProp Σ).
-	Context (srv_si : message → iProp Σ).
+	Context `{ IP : !@RPC_interface_params Σ }.
 	Notation srv_ip := (ip_of_address RPC_saddr).
+	
+
 
 	Definition req_prot_aux (rec : iProto Σ) : iProto Σ :=
-		(<! (UP : RPC_handler_user_params) (req : val) (s_arg : string) (argv : val) (argd : RPC_arg_data) >
-			MSG req {{ ⌜req = (#UP.(RPC_name), #s_arg)%V ∧ s_is_ser RPC_arg_ser argv s_arg⌝ ∗ RPC_handler_pre argv argd }} ;
-		<? (s_rep : string) (repv : val) (repd : RPC_rep_data) >
-			MSG #s_rep {{ ⌜s_is_ser RPC_rep_ser repv s_rep⌝ ∗ RPC_handler_post repv argd repd }};
+		(<! (RP : RPC_rpc_params) (s_arg : string) (arg : val) (argd : RP.(RPC_arg_data)) >
+			MSG (#RP.(RPC_name), #s_arg)%V 
+			{{ ⌜In RP IP.(RPC_inter)⌝ ∗ ⌜s_is_ser RP.(RPC_arg_ser) arg s_arg⌝ ∗ RP.(RPC_pre) arg argd }} ;
+		<? (s_rep : string) (rep : val) (repd : RP.(RPC_rep_data)) >
+			MSG #s_rep 
+			{{ ⌜s_is_ser RP.(RPC_rep_ser) rep s_rep⌝ ∗ RP.(RPC_post) rep argd repd }};
 		rec)%proto.
 
 	Instance req_prot_aux_contractive : Contractive (req_prot_aux).
@@ -58,135 +60,347 @@ Section RPC_proof_of_code.
 	Context `{HspecS : !Reliable_communication_Specified_API_session cmh}.
 	Context `{HspecN : !Reliable_communication_Specified_API_network MT_UP SnRes}.
 
-  Definition is_val_of_serialization (seria_val : val) (seria : serialization) : Prop :=
-	  ∃ ser_val deser_val,
-	  seria_val = (ser_val, deser_val)%V ∧ 
-		ser_val = s_ser (s_serializer seria) ∧ deser_val = s_deser (s_serializer seria).
+	Definition call_handler_spec (RP : RPC_rpc_params) (II : RPC_interface_implementation IP) : iProp Σ :=
+		{{{ ⌜In RP IP.(RPC_inter)⌝ }}}
+			call_handler II.(RPC_inter_val) #RP.(RPC_name) @[srv_ip]
+		{{{ h, RET h; ⌜is_impl_handler_of_rpc h RP⌝ }}}.
 
-  Definition s_call_spec `{UP: !RPC_handler_user_params} (name : val) (s_handler : val): iProp Σ :=
-		⌜#RPC_name = name⌝ →
-		∀ argd argv s_arg (mon : val),
-		{{{ ⌜s_is_ser RPC_arg_ser argv s_arg⌝ ∗ RPC_handler_pre argv argd }}}
-			s_handler mon #s_arg @[srv_ip]
-		{{{ repd repv (s_rep : string), RET #s_rep; ⌜s_is_ser RPC_rep_ser repv s_rep⌝ ∗ RPC_handler_post repv argd repd }}}.
-
-	(*Definition handler_spec `{UP: !RPC_handler_user_params} (handler : val) : iProp Σ :=
-		∀ argd argv (mon : val),
-		{{{ RPC_handler_pre argv argd }}}
-			handler mon argv @[srv_ip]
-		{{{ repd repv, RET repv; RPC_handler_post repv argd repd ∗ ⌜Serializable RPC_rep_ser repv⌝ }}}.*)
-
- 	(* Definition implement_spec `{UP : !RPC_handler_user_params} : iProp Σ :=
-		∀ (rpc : val) handler name ser1 ser2,
-		⌜rpc = (name, (ser1, ser2))%V⌝ ∧
-		⌜name = #RPC_name⌝ ∧ 
-		⌜is_val_of_serialization ser1 RPC_arg_ser ∧ is_val_of_serialization ser2 RPC_rep_ser⌝ -∗
-		{{{ handler_spec handler }}}
-			implement rpc handler @[srv_ip]
-		{{{ v s_handler, RET v; ⌜v = (name, s_handler)%V⌝ ∗ s_call_spec name s_handler }}}.
-
-	Lemma implement_spec_holds `{UP : !RPC_handler_user_params} : ⊢ implement_spec.
+	Lemma call_handler_spec_holds (RP : RPC_rpc_params) (II : RPC_interface_implementation IP) :
+		⊢ call_handler_spec RP II.
 	Proof.
-		iIntros (rpc handler name ser1 ser2 Hrpc Φ). iModIntro. iIntros "#Hspec Hcont".
-		rewrite /implement. wp_pures.
-		destruct Hrpc as [-> [-> [Hser1 Hser2]]]. wp_pures.
-		iApply "Hcont". iSplitL; try done.
-		rewrite /s_call_spec. iIntros "_". iIntros (argd argv s_arg mon Ψ). iModIntro. iIntros "[%Hser Hpre] Hcont".
+		rewrite /call_handler_spec.
+		iIntros (Φ). iModIntro. iIntros "%HRP Hcont".
+		rewrite /call_handler.
+		wp_pures. iApply "Hcont".
+		iPureIntro. rewrite /is_impl_handler_of_rpc.
+		iIntros (argv argd s_arg Ψ) "[%Hargser Hpre] Hcont".
+		wp_pures. wp_lam. wp_pure _.
+		iAssert 
+		(
+			(∀ (inter : val),
+			(∃ (inter_list : list val) (inter_params : list RPC_rpc_params),
+			⌜is_list inter_list inter ∧
+			is_list_of_interface inter_list inter_params ∧
+			List.NoDup (map (fun RP => RP.(RPC_name)) inter_params) ∧
+			In RP inter_params⌝) -∗
+			WP let: "func" := network_util_code.unSOME
+                    ((rec: "loop" "m" :=
+                        match: "m" with
+                          InjL <> => InjL #()
+                        | InjR "p" =>
+                          if: Fst (Fst "p") =
+                              #RP.(RPC_name)
+                          then InjR (Snd (Fst "p"))
+                          else "loop" (Snd "p")
+                        end)%V inter) in
+   			"func" #s_arg @[srv_ip] {{ v, Ψ v }})%I
+		) with "[Hpre Hcont]" as "Hassert".
+		2 : 
+		{
+			iApply "Hassert".
+			iExists RPC_inter_list, IP.(RPC_inter).
+			iPureIntro. split.
+			apply RPC_inter_spec. split.
+			apply RPC_inter_spec. split.
+			apply RPC_inter_nodup. apply HRP.
+		}
+		iLöb as "IH".
+		iIntros (inter) "H".
+		iDestruct "H" as (inter_list inter_params) "(%Hlist & %Hlistof & %Hnodup & %Hin)".
+		destruct inter_params as [| RP' inter']; first contradiction.
+		destruct inter_list; first contradiction.
+		simpl in Hlist. destruct Hlist as [l' [-> Hlist]].
+		destruct v; try contradiction.
+		destruct Hlistof as [-> [Hhand Hlistof]]. 
+
+		destruct Hin as [-> | Hin].
+		- wp_pures.
+		  case_bool_decide; last contradiction.
+		  rewrite /network_util_code.unSOME. wp_pures.
+		  wp_apply (Hhand with "[$Hpre]"); first done.
+		  iApply "Hcont".
+		- wp_pures.
+		  case_bool_decide as Hnameeq.
+		  { assert (RP.(RPC_name) = RP'.(RPC_name)) as Heq.
+		  	{ by inversion Hnameeq. }  
+		  	simpl in Hnodup. apply (NoDup_cons_iff RPC_name _) in Hnodup. 
+			destruct Hnodup as [Hnotin _].
+			apply (@in_map _ _ (λ RP : RPC_rpc_params, RP.(RPC_name)) _ _) in Hin.
+			rewrite Heq in Hin. contradiction.
+		  }
+		  wp_if. wp_proj. 
+		  iApply ("IH" with "[$Hpre] [$Hcont]").
+		  iExists inter_list, inter'. iPureIntro.
+		  split. assumption.
+		  split. assumption.
+		  split.
+		  simpl in Hnodup. inversion Hnodup.
+		  assumption. assumption.
+	Qed.
+
+	Lemma service_loop_proof (II : RPC_interface_implementation IP) (c : val) :
+		{{{ c ↣{ ip_of_address RPC_saddr, string_serialization } iProto_dual req_prot }}}
+		service_loop c II.(RPC_inter_val) #() @[srv_ip]
+		{{{ RET #(); ⌜True⌝ }}}.
+	Proof.
+		iIntros (Φ) "Hc Hcont".
+		rewrite /service_loop. do 8 wp_pure _.
+		iLöb as "IH".
 		wp_pures.
-		destruct Hser1 as [ser_val [deser_val [-> [-> ->]]]]. wp_pures.
-		wp_apply (s_deser_spec RPC_arg_ser). iPureIntro. apply Hser. iIntros "_".
+		wp_recv (rpc s_arg arg argd) as "(%Hin & Hser & Hpre)".
 		wp_pures.
-		destruct Hser2 as [ser_val [deser_val [-> [-> ->]]]]. 
-		wp_apply ("Hspec" with "[$Hpre]").
-		iIntros (repd repv) "[Hpost %Hrep]".
-		wp_pures.
-		wp_apply (s_ser_spec RPC_rep_ser).
-		{ iPureIntro. apply Hrep. }
+		(* wp_apply (monitor_acquire_spec with "[Hmon]"); first by iFrame "#".
+		iIntros (v) "(-> & Hlocked & HR)". wp_seq. *)
+		wp_apply (call_handler_spec_holds); first by iFrame "#".
+		iIntros (h Hh). rewrite /is_impl_handler_of_rpc.
+		wp_apply (Hh with "[$Hpre $Hser]").
+		iIntros (repv repd s_rep) "[Hser Hpost]".
+		wp_let.
+		(* wp_apply (monitor_release_spec with "[$Hmon $HR $Hlocked]").
+		iIntros (v ->). wp_seq. *)
+		wp_send with "[$Hser $Hpost]". wp_seq.
+		iApply ("IH" with "[$Hc] [$Hcont]").
+	Qed.
+		
+		
+		
+
+	Lemma accept_new_connections_loop_proof (II : RPC_interface_implementation IP) skt  :
+		{{{ RPC_saddr ⤇ reserved_server_socket_interp ∗
+			SrvListens skt }}}
+		accept_new_connections_loop skt II.(RPC_inter_val) #() @[srv_ip]
+		{{{ RET #(); False }}}.
+	Proof.
+		iIntros (Φ) "[#Hsi Hlistens] Hcont".
+		rewrite /accept_new_connections_loop.
+		do 8 wp_pure _.
+		iLöb as "IH". wp_pure _.
+		wp_smart_apply (RCSpec_accept_spec with "[$Hlistens]").
+		iIntros (c client_addr v) "(-> & Hlistens & Hc)". wp_pures.
+		wp_apply (aneris_wp_fork with "[-]").
+		iSplitL "Hlistens".
+		- iNext.
+			do 2 wp_pure _.
+			iApply ("IH" with "[$Hlistens]").
+			by iIntros.
+		- iNext.
+			wp_pures.
+			simpl in *.
+			by wp_apply (service_loop_proof with "[$Hc]").
+		Qed.
+
+	Definition init_server_stub_internal_spec (II : RPC_interface_implementation IP) : iProp Σ :=
+		∀ A,
+		{{{ ⌜RPC_saddr ∈ A⌝ ∗
+				fixed A ∗
+				free_ports (ip_of_address RPC_saddr) {[port_of_address RPC_saddr]} ∗
+				RPC_saddr ⤇ reserved_server_socket_interp ∗
+				RPC_saddr ⤳ (∅, ∅) ∗
+				SrvInit }}}
+			init_server_stub #RPC_saddr II.(RPC_inter_val) @[srv_ip]
+		{{{ RET #(); ⌜False⌝ }}}.
+
+	Lemma init_server_stub_internal_spec_holds (II : RPC_interface_implementation IP) :
+		⊢ init_server_stub_internal_spec II.
+	Proof.
+		iIntros (A Φ) "!#". 
+		iIntros "(#HA & #Hfix & Hfp & #Hsi & Hhist & Hinit) Hcont".
+		rewrite /init_server_stub. wp_pures.
+		wp_apply (RCSpec_make_server_skt_spec with "[$HA $Hhist $Hsi $Hfix $Hinit $Hfp] [Hcont]").
+		iNext. iIntros (skt) "Hcl". wp_pures.
+		wp_apply (RCSpec_server_listen_spec with "[$Hcl] [Hcont]").
+		iNext. iIntros (v) "[-> Hlistens]". wp_seq.
+		wp_apply (accept_new_connections_loop_proof with "[$]").
+		iApply "Hcont".
+	Qed.
+
+
+
+
+	Definition implement_spec {RP : RPC_rpc_params} (IMP : RPC_implementation_params RP) : iProp Σ :=
+		{{{ ⌜In RP IP.(RPC_inter)⌝ }}}
+			implement IMP.(RPC_val) IMP.(RPC_handler) @[srv_ip]
+		{{{ h, RET (#RP.(RPC_name), h)%V; ⌜is_impl_handler_of_rpc h RP⌝ }}}.
+
+	Lemma implement_spec_holds {RP : RPC_rpc_params} (IMP : RPC_implementation_params RP) : 
+		⊢ implement_spec IMP.
+	Proof.
+		iIntros (Φ) "!#". iIntros (HRP) "Hcont".
+		rewrite /implement.
+		rewrite RPC_rpc_match. wp_pures.
+		iApply "Hcont". iPureIntro.
+		rewrite /is_impl_handler_of_rpc.
+		iIntros (argv argd s_arg Ψ) "[%Hargser Hpre] Hcont".
+		wp_pures. wp_apply (s_deser_spec RPC_arg_ser); first done.
+		iIntros "_". wp_pures.
+		wp_apply (RPC_handler_spec with "Hpre").
+		iIntros (repv repd) "[%Hseria Hpost]". wp_pures.
+		wp_apply (s_ser_spec RPC_rep_ser); first done.
 		iIntros (s Hrepser). iApply "Hcont".
-		iFrame. done.
-	Qed. *)
+		by iFrame.
+	Qed.
 
-	(* spécification de ce qui est obtenu quand on fait "call chan aRPC"
-	Definition user_handler_spec `{UP : !RPC_handler_user_params} handler clt_addr : iProp Σ :=
-		∀ argv argd,
-		{{{ ⌜Serializable RPC_arg_ser argv⌝ ∗ RPC_handler_pre argv argd }}}
-			handler argv @[ip_of_address clt_addr]
-		{{{ repv repd, RET repv; RPC_handler_post repv argd repd }}}. *)
-
-	Definition LockedChannel (chan : val) clt_addr : iProp Σ :=
-		∃ c lk (γ : gname), ⌜chan = (c, lk)%V⌝ ∧ 
-		is_lock (RPC_mN.@"proxy") (ip_of_address clt_addr) γ lk
-			(c ↣{ip_of_address clt_addr,RCParams_clt_ser} RCParams_protocol).
-
-	Definition init_client_stub_spec A clt_addr : iProp Σ :=
-		{{{ ⌜clt_addr ∉ A⌝ ∗ fixed A ∗ free_ports (ip_of_address clt_addr) {[port_of_address clt_addr]} ∗
-			clt_addr ⤳ (∅, ∅) ∗ RPC_saddr ⤇ reserved_server_socket_interp }}}
+	Definition init_client_stub_internal_spec : iProp Σ :=
+		∀ A clt_addr,
+		{{{ ⌜clt_addr ∉ A⌝ ∗ 
+				fixed A ∗ 
+				free_ports (ip_of_address clt_addr) {[port_of_address clt_addr]} ∗
+				clt_addr ⤳ (∅, ∅) ∗ 
+				RPC_saddr ⤇ reserved_server_socket_interp }}}
 			init_client_stub #clt_addr #RPC_saddr @[ip_of_address clt_addr]
-		{{{ chan, RET chan; LockedChannel chan clt_addr }}}.
+		{{{ chan, RET chan; chan ↣{ip_of_address clt_addr,RCParams_clt_ser} RCParams_protocol }}}.
 
-	Lemma init_client_stub_spec_holds A clt_addr : ⊢ init_client_stub_spec A clt_addr.
+	Lemma init_client_stub_internal_spec_holds : ⊢ init_client_stub_internal_spec.
 	Proof.
-		rewrite /init_client_stub_spec.
-		iIntros (Φ) "!#". iIntros "(#Hna & #Hfix & Hfp & Hhist & #Hsi) Hcont".
+		rewrite /init_client_stub_internal_spec.
+		iIntros (A clt_addr Φ) "!#". iIntros "(#Hna & #Hfix & Hfp & Hhist & #Hsi) Hcont".
 		rewrite /init_client_stub. wp_pures.
 		wp_apply (RCSpec_make_client_skt_spec with "[$Hfix $Hfp $Hhist $Hsi]"). iAssumption.
 		iIntros (skt) "Hcl". wp_pures.
 		wp_apply (RCSpec_connect_spec with "[$Hcl]").
 		iIntros (c) "Hcl". wp_pures.
-		wp_apply (newlock_spec
-					 (RPC_mN .@ "proxy") _
-					 ( c ↣{ip_of_address clt_addr,RCParams_clt_ser} RCParams_protocol) with "[$Hcl]").
-		iIntros (lk γ) "#Hlk". wp_pures.
-		iApply "Hcont".
-		iExists c, lk, γ. iFrame "#". done.
+		by iApply "Hcont".
 	Qed.
 
-	Definition call_spec `{UP : !RPC_handler_user_params} clt_addr : iProp Σ :=
-		∀ chan arg_ser rep_ser,
-		⌜is_val_of_serialization arg_ser RPC_arg_ser ∧ is_val_of_serialization rep_ser RPC_rep_ser⌝ -∗
-		∀ argv argd,
-		{{{ ⌜Serializable RPC_arg_ser argv⌝ ∗ RPC_handler_pre argv argd ∗ LockedChannel chan clt_addr }}}
-			call chan (#RPC_name, (arg_ser, rep_ser))%V argv @[ip_of_address clt_addr]
-		{{{ repv repd, RET repv; RPC_handler_post repv argd repd }}}.
+	Definition call_internal_spec {RP : RPC_rpc_params} (IMP : RPC_implementation_params RP) : iProp Σ :=
+		∀ chan clt_addr argv argd,
+		{{{ ⌜In RP IP.(RPC_inter)⌝ ∗ 
+			chan ↣{ip_of_address clt_addr,RCParams_clt_ser} RCParams_protocol ∗
+			⌜Serializable RP.(RPC_arg_ser) argv⌝ ∗ 
+			RP.(RPC_pre) argv argd }}}
+			call chan IMP.(RPC_val) argv @[ip_of_address clt_addr]
+		{{{ repv repd, RET repv; 
+			chan ↣{ip_of_address clt_addr,RCParams_clt_ser} RCParams_protocol ∗
+			RP.(RPC_post) repv argd repd }}}.
 
-	Lemma call_spec_holds `{UP : !RPC_handler_user_params} clt_addr : ⊢ call_spec clt_addr.
+	Lemma call_internal_spec_holds {RP : RPC_rpc_params} (IMP : RPC_implementation_params RP) :
+		⊢ call_internal_spec IMP.
 	Proof.
-		rewrite /call_spec.
-		iIntros (chan arg_ser rep_ser [Hargser Hrepser] argv argd Φ) "!#".
-		iIntros "(%Hser & Hpre & #Hlc) Hcont".
-		rewrite /call. 
-		iDestruct "Hlc" as (c lk γ ->) "Hlk". wp_pures.
-		destruct Hargser as [_ [_ [-> [-> ->]]]]. wp_pures. 
-		wp_apply (s_ser_spec RPC_arg_ser). {iPureIntro. apply Hser. }
-		iIntros (s Hisser). wp_pures.
-		wp_apply (acquire_spec with "[$Hlk]").
-		iIntros (?) "(-> & Hlocked & Hc)". wp_seq.
+		rewrite /call_internal_spec.
+		iIntros (chan clt_addr argv argd Φ) "!#".
+		iIntros "(%HRP & Hc & %Hseria & Hpre) Hcont".
+		rewrite /call. wp_pures.
+		rewrite RPC_rpc_match. wp_pures.
+		wp_apply s_ser_spec; first done.
+		iIntros (s Hisserarg). wp_pures.
+		wp_send with "[$Hpre]"; first done.
+		wp_seq.
+		wp_recv (s_rep repv repd) as "[%Hisserep Hpost]". wp_pures.
+		wp_apply s_deser_spec; first done.
+		iIntros "_". iApply "Hcont". iFrame.
+	Qed.
+
+
+
+	(* Definition rpc_spec {RP : RPC_rpc_params} (f : val) clt_addr : iProp Σ :=
+		∀ argv argd,
+		{{{ ⌜Serializable RP.(RPC_arg_ser) argv⌝ ∗ RP.(RPC_pre) argv argd }}}
+			f argv @[ip_of_address clt_addr]
+		{{{ repv repd, RET repv; RP.(RPC_post) repv argd repd }}}.
+
+	Definition call_internal_spec {RP : RPC_rpc_params} (IMP : RPC_implementation_params RP) : iProp Σ :=
+		∀ chan clt_addr,
+		{{{ ⌜In RP IP.(RPC_inter)⌝ ∗ chan ↣{ip_of_address clt_addr,RCParams_clt_ser} RCParams_protocol }}}
+			call chan IMP.(RPC_val) @[ip_of_address clt_addr]
+		{{{ f, RET f; @rpc_spec RP f clt_addr }}}.
+
+	Lemma call_internal_spec_holds {RP : RPC_rpc_params} (IMP : RPC_implementation_params RP) :
+		⊢ call_internal_spec IMP.
+	Proof.
+		rewrite /call_internal_spec.
+		iIntros (chan clt_addr Φ) "!#".
+		iIntros "[%HRP Hc] Hcont".
+		rewrite /call. wp_pures.
+		(* rewrite /rpc_spec. *)
+		iApply "Hcont".
+		rewrite /rpc_spec. 
+		iIntros (argv argd Ψ) "!> [%Hseria Hpre] Hcont".
+		(* iDestruct "Hc" as (c lk γ ->) "Hlk". wp_pures. *)
+		rewrite RPC_rpc_match. wp_pures.
+		wp_apply s_ser_spec; first done.
+		iIntros (s Hisserarg). wp_pures.
 		wp_send with "[$Hpre]"; first done.
 		wp_seq.
 		wp_recv (s_rep repv repd) as "[%Hisserep Hpost]". wp_pures.
 		wp_apply (release_spec with "[$Hlk $Hc $Hlocked]").
-		iIntros (? ->). wp_seq.
-		wp_pures. destruct Hrepser as [_ [_ [-> [-> ->]]]]. wp_pures.
-		wp_apply (s_deser_spec RPC_rep_ser); first done.
+		iIntros (? ->). wp_seq. wp_pures. 
+		wp_apply s_deser_spec; first done.
 		iIntros "_". by iApply "Hcont".
+	Qed. *)
+
+	Global Definition Channel chan clt_addr := chan ↣{ip_of_address clt_addr,RCParams_clt_ser} RCParams_protocol.
+
+End RPC_proof_of_code.
+
+From aneris.examples.reliable_communication.spec
+     Require Import ras.
+From aneris.examples.reliable_communication.instantiation
+     Require Import instantiation_of_init.
+From aneris.examples.reliable_communication.lib.reliable_rpc
+     Require Import api_spec.
+
+Section RPC_proof_of_init.
+	Context `{ !anerisG Mdl Σ, !lockG Σ}.
+	Context `{ !RPC_user_params }.
+	Context `{ IP : !@RPC_interface_params Σ }.
+	Context `{ !SpecChanG Σ }.
+
+	Lemma RPC_init_setup_holds (E : coPset) :
+	↑RPC_mN ⊆ E →
+    ⊢ |={E}=> ∃ (srv_si : message → iProp Σ) (SrvInit : iProp Σ)
+								(Channel : val → socket_address → iProp Σ),
+			SrvInit ∗
+			(∀ (II : RPC_interface_implementation IP), 
+				init_server_stub_spec SrvInit srv_si II) ∗
+			(init_client_stub_spec srv_si Channel) ∗
+			( ∀ (RP : RPC_rpc_params) (IMP : RPC_implementation_params RP),
+				@call_spec _ _ _ _ IP Channel RP IMP).
+	Proof.
+		iIntros (HE).
+		iMod (Reliable_communication_init_setup E MT_UP HE)
+      		as (chn sgn) "(Hinit & Hspecs)".
+		iDestruct "Hspecs"
+		as "(
+			%HmkClt & %HmkSrv
+			& %Hconnect
+			& %Hlisten & %Haccept
+			& %Hsend & %HsendTele
+			& %HtryRecv & %Hrecv)".
+		iExists reserved_server_socket_interp, SrvInit, Channel.
+		iFrame. iModIntro. iSplitL.
+		- iIntros (II). rewrite /init_server_stub_spec.
+			iIntros (A Φ) "!#".
+			iIntros "(#Hsi & Hfix & HA & Hhist & Hfp & Hinit) Hcont".
+			iApply (init_server_stub_internal_spec_holds with "[$HA $Hfix $Hfp $Hsi $Hhist $Hinit][$]").
+			Unshelve. done. done. done.
+		- iSplitL.
+			+ rewrite /init_client_stub_spec.
+				iIntros (A clt_addr Φ) "!#".
+				iIntros "(#Hsi & Hfix & HA & Hhist & Hfp) Hcont".
+				iApply (init_client_stub_internal_spec_holds with "[$HA $Hfix $Hfp $Hsi $Hhist][$]").
+				Unshelve. done.
+			+ iIntros (RP IMP). rewrite /call_spec.
+				iIntros (chan clt_addr argv argd Φ) "!#".
+				iIntros "(HRP & Hchan & Hseria & Hpre) Hcont".
+				iApply (call_internal_spec_holds IMP with "[$HRP $Hchan $Hseria $Hpre][$]").
+				Unshelve. done.
+		Qed.
+
+End RPC_proof_of_init.
+
+Section RPC_proof_of_init_class.
+	Context `{!anerisG Mdl Σ}.
+	Context `{!lockG Σ}.
+	Context `{!MTS_user_params}.
+	Context `{!SpecChanG Σ}.
+
+	Global Instance rpc_init : RPC_init.
+	Proof.
+		split. iIntros (E UP IP HE).
+		iMod (RPC_init_setup_holds E HE) as (srv_si SrvInit Channel) "[Hinit Hspecs]".
+		iModIntro.
+		iExists _, _, _. iFrame.
 	Qed.
 
-	Definition call_handler_spec : iProp Σ :=
-		⌜is_map handlers handlers_map⌝ -∗
-		{{{ 
-				is_monitor RPC_mN (ip_of_address RPC_saddr) RPC_mγ RPC_mv RPC_mR ∗
-				locked RPC_mγ ∗ RPC_mR ∗
-				RPC_handler_pre reqv reqd  }}}
-			call_handler handlers name s_arg
-		{{{ repv repd, RET repv;
-				⌜Serializable RPC_rep_ser repv⌝ ∗
-				locked RPC_mγ ∗ RPC_mR ∗
-				RPC_handler_post repv reqd repd }}}
-
-	Lemma service_loop_proof `{UP : !RPC_handler_user_params} (c : val) :
-    {{{ is_monitor RPC_mN (ip_of_address RPC_saddr) RPC_mγ RPC_mv RPC_mR ∗
-      c ↣{ ip_of_address RPC_saddr, RPC_rep_ser } iProto_dual req_prot  }}}
-      service_loop c RPC_mv RPC_handler #() @[ip_of_address RPC_saddr]
-    {{{ RET #(); ⌜True⌝  }}}.
-
+End RPC_proof_of_init_class.
 
